src/CCLPrimitives.v
@@ -4,91 +4,125 @@ Require Import AsyncDisk.
 Require Import Word.
 Require Import Hashmap.
 Require Import FunctionalExtensionality.
+Require Import Automation.
 
 Import CCLTactics.
 
 Section Primitives.
 
-  Context {St:StateTypes}.
-  Variable G:Protocol St.
+  Variable G:Protocol.
 
   Ltac begin_prim :=
     unfold cprog_spec, cprog_ok; simpl; intros;
-    repeat deex;
-    try match goal with
-        | [ H: context[let (n, m) := ?a in _] |- _ ] =>
-          let n := fresh n in
-          let m := fresh m in
-          destruct a as [m n];
-          simpl in *;
-          Automation.safe_intuition
-        end.
+    repeat deex.
 
-  Ltac inv_opt :=
+  Lemma if_CanWrite : forall A (a a':A) l,
+      l = WriteLock ->
+      (if CanWrite l then a else a') = a.
+  Proof.
+    intros.
+    subst; simpl; auto.
+  Qed.
+
+  Hint Rewrite if_CanWrite using (solve [ auto ]) : locks.
+
+  Ltac simplify_step :=
     match goal with
+    | [ H: context[let '(n, m) := ?a in _] |- _] =>
+      destruct a; simpl in *; intuition eauto
+    | [ H: precondition {| precondition := _; postcondition := _ |} |- _ ] =>
+      simpl in *; intuition eauto
+    | [ H: context[exec _ _ _ _ _ -> _] |-
+        match ?out with
+        | Finished _ _ _ => _
+        | Error => _
+        end ] => eapply H; eauto; simpl; intuition eauto
+    | [ H: ?F (Sigma.mem ?sigma) |- ?F (Sigma.mem _) ] =>
+      solve [ destruct sigma; simpl in H; apply H ]
+    | [ |- Sigma.disk (Sigma.upd_disk ?sigma _) = _ ] =>
+      destruct sigma; simpl in *
+    | [ |- Sigma.hm _ = Sigma.hm ?sigma ] =>
+      solve [ destruct sigma; simpl in *; auto ]
+    | [ |- Sigma.disk _ = Sigma.disk ?sigma ] =>
+      solve [ destruct sigma; simpl in *; auto ]
+    | [ |- Sigma.l _ = Sigma.l ?sigma ] =>
+      solve [ destruct sigma; simpl in *; auto ]
+    | [ H: (_ * ?a |-> ?v)%pred _ |- _ ] =>
+      learn that (ptsto_valid' H)
+    | [ H: ?a = ?b, H': ?a = ?b' |- _ ] =>
+      rewrite H in *; clear H
     | [ H: Some _ = Some _ |- _ ] =>
       inversion H; subst; clear H
+    | _ => simpl_match
+    | _ => progress autorewrite with locks in *
+    | [ x := _ |- _ ] => subst x
+    | _ => progress subst
+    | _ => auto; congruence
     end.
+
+  Ltac prim :=
+    begin_prim;
+    inv_bind; inv_exec;
+    unfold ident in *;
+    repeat inj_pair2;
+    repeat simplify_step.
 
   Theorem BeginRead_ok : forall tid a,
       cprog_spec G tid
-                 (fun v '(sigma_i, sigma) =>
+                 (fun '(F, v) '(sigma_i, sigma) =>
                     {| precondition :=
+                         F (Sigma.mem sigma) /\
                          Sigma.disk sigma a = Some (v, NoReader) /\
                          Sigma.l sigma = WriteLock;
                        postcondition :=
                          fun '(sigma_i', sigma') _ =>
+                           F (Sigma.mem sigma') /\
                            sigma_i' = sigma_i /\
-                           sigma' = Sigma.upd_disk sigma (fun d => upd d a (v, Pending)); |})
+                           Sigma.hm sigma' = Sigma.hm sigma /\
+                           Sigma.l sigma' = Sigma.l sigma /\
+                           Sigma.disk sigma' = upd (Sigma.disk sigma) a (v, Pending); |})
                  (BeginRead a).
   Proof.
-    begin_prim.
-    inv_bind; inv_exec.
-    inv_opt.
-
-    eapply H2; eauto; simpl.
-    intuition eauto.
+    prim.
   Qed.
 
   Theorem WaitForRead_ok : forall tid a,
       cprog_spec G tid
-                 (fun v '(sigma_i, sigma) =>
+                 (fun '(F, v) '(sigma_i, sigma) =>
                     {| precondition :=
+                         F (Sigma.mem sigma) /\
                          Sigma.disk sigma a = Some (v, Pending) /\
                          Sigma.l sigma = WriteLock;
                        postcondition :=
                          fun '(sigma_i', sigma') r =>
+                           F (Sigma.mem sigma') /\
                            sigma_i' = sigma_i /\
-                           sigma' = Sigma.upd_disk sigma (fun d => upd d a (v, NoReader)) /\
+                           Sigma.hm sigma' = Sigma.hm sigma /\
+                           Sigma.l sigma' = Sigma.l sigma /\
+                           Sigma.disk sigma' = upd (Sigma.disk sigma) a (v, NoReader) /\
                            r = v; |})
                  (WaitForRead a).
   Proof.
-    begin_prim.
-    inv_bind; inv_exec.
-    inv_opt.
-
-    eapply H2; eauto; simpl.
-    intuition eauto.
+    prim.
   Qed.
 
   Theorem Write_ok : forall tid a v,
       cprog_spec G tid
-                 (fun v0 '(sigma_i, sigma) =>
+                 (fun '(F, v0) '(sigma_i, sigma) =>
                     {| precondition :=
+                         F (Sigma.mem sigma) /\
                          Sigma.disk sigma a = Some (v0, NoReader) /\
                          Sigma.l sigma = WriteLock;
                        postcondition :=
                          fun '(sigma_i', sigma') _ =>
+                           F (Sigma.mem sigma') /\
                            sigma_i' = sigma_i /\
-                           sigma' = Sigma.upd_disk sigma (fun d => upd d a (v, NoReader)); |})
+                           Sigma.hm sigma' = Sigma.hm sigma /\
+                           Sigma.disk sigma' =  upd (Sigma.disk sigma) a (v, NoReader) /\
+                           Sigma.l sigma' = Sigma.l sigma; |})
                  (Write a v).
   Proof.
-    begin_prim.
-    inv_bind; inv_exec.
-    inv_opt.
-
-    eapply H2; eauto; simpl.
-    intuition eauto.
+    prim.
   Qed.
 
   Lemma read_permission_not_free : forall l,
@@ -102,58 +136,83 @@ Section Primitives.
 
   Hint Resolve read_permission_not_free.
 
-  Theorem Get_ok : forall tid,
+  Theorem Alloc_ok : forall tid A (v:A),
       cprog_spec G tid
-                 (fun (_:unit) '(sigma_i, sigma) =>
-                    {| precondition := ReadPermission (Sigma.l sigma);
+                 (fun F '(sigma_i, sigma) =>
+                    {| precondition :=
+                         F (Sigma.mem sigma) /\
+                         Sigma.l sigma = WriteLock;
                        postcondition :=
-                         fun  '(sigma_i', sigma') r =>
-                           sigma_i' = sigma_i /\
-                           sigma' = sigma /\
-                           r = Sigma.mem sigma; |})
-                 Get.
+                         fun '(sigma_i', sigma') i =>
+                           ((F:heappred) * i |-> val v)%pred (Sigma.mem sigma') /\
+                           Sigma.disk sigma' = Sigma.disk sigma /\
+                           Sigma.hm sigma' = Sigma.hm sigma /\
+                           Sigma.l sigma' = Sigma.l sigma /\
+                           sigma_i' = sigma_i; |})
+                 (Alloc v).
   Proof.
-    begin_prim.
-    inv_bind; inv_exec; eauto.
-
-    eapply H2; eauto; simpl.
-    intuition eauto.
+    prim.
+    destruct sigma; simpl in *.
+    eapply ptsto_upd_disjoint; eauto.
   Qed.
 
-  Theorem Assgn_ok : forall tid m',
+  Theorem Get_ok : forall tid A i,
       cprog_spec G tid
-                 (fun (_:unit) '(sigma_i, sigma) =>
-                    {| precondition := Sigma.l sigma = WriteLock;
+                 (fun '(F, v0) '(sigma_i, sigma) =>
+                    {| precondition :=
+                         ((F:heappred) * i |-> val (v0:A))%pred (Sigma.mem sigma) /\
+                         ReadPermission (Sigma.l sigma);
+                       postcondition :=
+                         fun '(sigma_i', sigma') r =>
+                           sigma' = sigma /\
+                           r = v0; |})
+                 (Get A i).
+  Proof.
+    prim.
+
+    inj_pair2; auto.
+    inv_exec; eauto.
+  Qed.
+
+  Theorem Assgn_ok : forall tid A i (v:A),
+      cprog_spec G tid
+                 (fun '(F, v0) '(sigma_i, sigma) =>
+                    {| precondition :=
+                         ((F:heappred) * i |-> val (v0:A))%pred (Sigma.mem sigma) /\
+                         Sigma.l sigma = WriteLock;
                        postcondition :=
                          fun '(sigma_i', sigma') _ =>
+                           (F * i |-> val v)%pred (Sigma.mem sigma') /\
                            sigma_i' = sigma_i /\
-                           sigma' = Sigma.set_mem sigma m'; |})
-                 (Assgn m').
+                           Sigma.hm sigma' = Sigma.hm sigma /\
+                           Sigma.disk sigma' = Sigma.disk sigma /\
+                           Sigma.l sigma' = Sigma.l sigma; |})
+                 (Assgn i v).
   Proof.
-    begin_prim.
-    inv_bind; inv_exec.
-
-    eapply H2; eauto; simpl.
-    intuition eauto.
+    prim.
+    inj_pair2.
+    destruct sigma; simpl in *; eauto.
+    eauto using ptsto_upd'.
   Qed.
 
   Theorem Hash_ok : forall tid sz (buf: word sz),
       cprog_spec G tid
-                 (fun (_:unit) '(sigma_i, sigma) =>
-                    {| precondition := True;
+                 (fun F '(sigma_i, sigma) =>
+                    {| precondition :=
+                         F (Sigma.mem sigma);
                        postcondition :=
                          fun '(sigma_i', sigma') r =>
+                           F (Sigma.mem sigma') /\
                            r = hash_fwd buf /\
                            hash_safe (Sigma.hm sigma) (hash_fwd buf) buf /\
                            sigma_i' = sigma_i /\
-                           sigma' = Sigma.upd_hm sigma buf; |})
+                           Sigma.disk sigma' = Sigma.disk sigma /\
+                           Sigma.hm sigma' = upd_hashmap' (Sigma.hm sigma) (hash_fwd buf) buf /\
+                           Sigma.l sigma' = Sigma.l sigma; |})
                  (Hash buf).
   Proof.
-    begin_prim.
-    inv_bind; inv_exec.
-
-    eapply H2; eauto; simpl.
-    intuition eauto.
+    prim.
+    destruct sigma; eauto.
   Qed.
 
   Theorem Ret_ok : forall tid T (v:T),
@@ -167,43 +226,64 @@ Section Primitives.
                            r = v; |})
                  (Ret v).
   Proof.
-    begin_prim.
-    inv_bind; inv_exec.
-
-    eapply H2; eauto; simpl.
-    intuition eauto.
+    prim.
   Qed.
 
-  Theorem GhostUpdate_ok : forall tid up,
+  Theorem GhostUpdate_ok : forall tid A i up,
       cprog_spec G tid
-                 (fun (_:unit) '(sigma_i, sigma) =>
-                    {| precondition := Sigma.l sigma = WriteLock;
+                 (fun '(F, v0) '(sigma_i, sigma) =>
+                    {| precondition :=
+                         ((F:heappred) * i |-> abs (v0:A))%pred (Sigma.mem sigma) /\
+                         Sigma.l sigma = WriteLock;
                        postcondition :=
                          fun '(sigma_i', sigma') _ =>
+                           (F * i |-> abs (up tid v0))%pred (Sigma.mem sigma') /\
                            sigma_i' = sigma_i /\
-                           sigma' = Sigma.upd_s sigma (up tid); |})
-                 (GhostUpdate up).
+                           Sigma.hm sigma' = Sigma.hm sigma /\
+                           Sigma.disk sigma' = Sigma.disk sigma /\
+                           Sigma.l sigma' = Sigma.l sigma; |})
+                 (GhostUpdate i up).
   Proof.
-    begin_prim.
-    inv_bind; inv_exec.
-
-    eapply H2; eauto; simpl.
-    intuition eauto.
+    prim.
+    inj_pair2.
+    destruct sigma; simpl in *.
+    eauto using ptsto_upd'.
   Qed.
 
-  Definition GetReadLock : @cprog St _ :=
+  Theorem GhostUpdateMem_ok : forall tid A AEQ V i up,
+      cprog_spec G tid
+                 (fun '(F, m0) '(sigma_i, sigma) =>
+                    {| precondition :=
+                         ((F:heappred) * i |-> absMem (m0:@mem A AEQ V))%pred (Sigma.mem sigma) /\
+                         Sigma.l sigma = WriteLock;
+                       postcondition :=
+                         fun '(sigma_i', sigma') _ =>
+                           (F * i |-> absMem (up tid m0))%pred (Sigma.mem sigma') /\
+                           sigma_i' = sigma_i /\
+                           Sigma.hm sigma' = Sigma.hm sigma /\
+                           Sigma.disk sigma' = Sigma.disk sigma /\
+                           Sigma.l sigma' = Sigma.l sigma; |})
+                 (GhostUpdateMem i up).
+  Proof.
+    prim.
+    repeat inj_pair2.
+    destruct sigma; simpl in *.
+    eauto using ptsto_upd'.
+  Qed.
+
+  Definition GetReadLock :=
     SetLock Free ReadLock.
 
-  Definition GetWriteLock : @cprog St _ :=
+  Definition GetWriteLock :=
     SetLock Free WriteLock.
 
-  Definition UpgradeReadLock : @cprog St _ :=
+  Definition UpgradeReadLock :=
     SetLock ReadLock WriteLock.
 
-  Definition ReleaseReadLock : @cprog St _ :=
+  Definition ReleaseReadLock :=
     SetLock ReadLock Free.
 
-  Definition Unlock : @cprog St _ :=
+  Definition Unlock :=
     SetLock WriteLock Free.
 
   Theorem GetReadLock_ok : forall tid,
@@ -218,12 +298,7 @@ Section Primitives.
                                  sigma_i' = sigma''; |})
                  GetReadLock.
   Proof.
-    begin_prim.
-    inv_bind; inv_exec.
-
-    eapply H2; eauto.
-    intuition eauto.
-
+    prim.
     eexists; intuition eauto.
     destruct sigma'0; simpl; eauto.
   Qed.
@@ -240,15 +315,12 @@ Section Primitives.
                                  sigma_i' = sigma''; |})
                  GetWriteLock.
   Proof.
-    begin_prim.
-    inv_bind; inv_exec.
-
-    eapply H2; eauto.
-    intuition eauto.
-
+    prim.
     eexists; intuition eauto.
     destruct sigma'0; simpl; eauto.
   Qed.
+
+  (* TODO: change these to separation logic style specs *)
 
   Theorem UpgradeReadLock_ok : forall tid,
       cprog_spec G tid
@@ -263,14 +335,7 @@ Section Primitives.
                            end; |})
                  UpgradeReadLock.
   Proof.
-    begin_prim.
-    inv_bind; inv_exec.
-
-    eapply H2; eauto.
-    intuition eauto.
-
-    eapply H2; eauto.
-    intuition eauto.
+    prim.
   Qed.
 
   Theorem ReleaseReadLock_ok : forall tid,
@@ -283,11 +348,7 @@ Section Primitives.
                            sigma_i' = sigma_i; |})
                  ReleaseReadLock.
   Proof.
-    begin_prim.
-    inv_bind; inv_exec.
-
-    eapply H2; eauto.
-    intuition eauto.
+    prim.
   Qed.
 
   Theorem Unlock_ok : forall tid,
@@ -301,11 +362,9 @@ Section Primitives.
                            sigma_i' = sigma'; |})
                  Unlock.
   Proof.
-    begin_prim.
-    inv_bind; inv_exec.
-
-    eapply H2; eauto.
-    intuition eauto.
+    prim.
+    destruct (lock_dec (Sigma.l sigma) WriteLock); try congruence.
+    destruct (lock_dec (Sigma.l sigma) ReadLock); try congruence.
   Qed.
 
 End Primitives.
@@ -313,11 +372,13 @@ End Primitives.
 Hint Extern 0 {{ BeginRead _; _ }} => apply BeginRead_ok : prog.
 Hint Extern 0 {{ WaitForRead _; _ }} => apply WaitForRead_ok : prog.
 Hint Extern 0 {{ Write _ _; _ }} => apply Write_ok : prog.
-Hint Extern 0 {{ @Get _; _ }} => apply @Get_ok : prog.
-Hint Extern 0 {{ Assgn _; _ }} => apply Assgn_ok : prog.
+Hint Extern 0 {{ Alloc _; _ }} => apply Alloc_ok : prog.
+Hint Extern 0 {{ Get _ _; _ }} => apply Get_ok : prog.
+Hint Extern 0 {{ Assgn _ _; _ }} => apply Assgn_ok : prog.
 Hint Extern 0 {{ Hash _; _ }} => apply Hash_ok : prog.
 Hint Extern 0 {{ Ret _; _ }} => apply Ret_ok : prog.
-Hint Extern 0 {{ GhostUpdate _; _ }} => apply GhostUpdate_ok : prog.
+Hint Extern 0 {{ GhostUpdate _ _; _ }} => apply GhostUpdate_ok : prog.
+Hint Extern 0 {{ GhostUpdateMem _ _; _ }} => apply GhostUpdateMem_ok : prog.
 Hint Extern 0 {{ GetReadLock; _ }} => apply GetReadLock_ok : prog.
 Hint Extern 0 {{ GetWriteLock; _ }} => apply GetWriteLock_ok : prog.
 Hint Extern 0 {{ UpgradeReadLock; _ }} => apply UpgradeReadLock_ok : prog.
