src/SyncRead.v
@@ -4,48 +4,62 @@ Require Import FunctionalExtensionality.
 
 Section SyncRead.
 
-  Variable St:StateTypes.
-  Variable G: Protocol St.
+  Variable G: Protocol.
 
-  Definition SyncRead a : @cprog St _ :=
+  Definition SyncRead a :=
     _ <- BeginRead a;
       v <- WaitForRead a;
       Ret v.
 
+  Ltac break_tuple a n m :=
+    let n := fresh n in
+    let m := fresh m in
+    destruct a as [n m];
+    simpl in *.
+
   Theorem SyncRead_ok : forall tid a,
       cprog_spec G tid
-                 (fun v0 '(sigma_i, sigma) =>
+                 (fun '(F, v0) '(sigma_i, sigma) =>
                     {| precondition :=
+                         F (Sigma.mem sigma) /\
                          Sigma.l sigma = WriteLock /\
                          Sigma.disk sigma a = Some (v0, NoReader);
                        postcondition :=
                          fun '(sigma_i', sigma') r =>
+                           F (Sigma.mem sigma') /\
                            sigma_i' = sigma_i /\
-                           sigma' = sigma /\
+                           Sigma.hm sigma' = Sigma.hm sigma /\
+                           Sigma.disk sigma' = Sigma.disk sigma /\
                            r = v0; |})
                  (SyncRead a).
   Proof.
     unfold SyncRead.
-    step.
+    step;
+      repeat match goal with
+             | [ H: context[let '(n, m) := ?a in _] |- _ ] =>
+               break_tuple a n m
+             end; intuition.
+    descend; simpl; intuition eauto.
 
-    eexists; intuition eauto.
+    step;
+      repeat match goal with
+             | [ H: context[let '(n, m) := ?a in _] |- _ ] =>
+               break_tuple a n m
+             end; intuition.
+    descend; simpl; intuition eauto.
 
-    step.
-
-    eexists; intuition eauto.
-
-    (* need better way to simplify nested updates on Sigma *)
-    destruct sigma; simpl in *.
+    replace (Sigma.disk sigma').
     autorewrite with upd; eauto.
+    congruence.
 
-    destruct sigma; simpl in *; auto.
+    step;
+      repeat match goal with
+             | [ H: context[let '(n, m) := ?a in _] |- _ ] =>
+               break_tuple a n m
+             end; intuition; try congruence.
+    replace (Sigma.disk sigma0).
+    replace (Sigma.disk sigma').
 
-    step.
-    intuition auto; simplify.
-
-    destruct sigma; simpl in *.
-
-    f_equal.
     extensionality a'.
     destruct (addr_eq_dec a a'); subst;
       autorewrite with upd; auto.
@@ -54,3 +68,7 @@ Section SyncRead.
 End SyncRead.
 
 Hint Extern 0 {{ SyncRead _; _ }} => apply SyncRead_ok : prog.
+
+(* Local Variables: *)
+(* company-coq-local-symbols: (("Sigma" . ?Σ) ("sigma" . ?σ) ("sigma'" . (?σ (Br . Bl) ?'))) *)
+(* End: *)
